---
layout: post
title: Elementary Classical Analysis - 1.14
tags: [Analysis]
---
## Problem

[a] Prove the [Lagrange's identity](https://en.wikipedia.org/wiki/Lagrange%27s_identity)

$$
(\sum\limits_{i=1}^{n} x_iy_i)^2 = (\sum\limits_{i=1}^{n} x_{i}^{2})\times(\sum\limits_{i=1}^{n} y_{i}^{2})-(\sum\limits_{1\leq i < j \leq n } x_iy_j - x_jy_i)^2
$$

and use this to give another proof of the [Cauchy-Schwarz inequality](https://en.wikipedia.org/wiki/Cauchy%E2%80%93Schwarz_inequality).

[b] Show that

$$
\sqrt{\sum\limits_{i=1}^{n}(x_i+y_i)^2}\leq \sqrt{\sum\limits_{i=1}^{n} x_{i}^{2}}+\sqrt{\sum\limits_{i=1}^{n} y_{i}^{2}}
$$

## Solution
 
**Answer[a]**

Use induction.

Note [Cauchy-Schwarz inequality](https://en.wikipedia.org/wiki/Cauchy%E2%80%93Schwarz_inequality) is

$$
(\sum\limits_{i=1}^{n} x_iy_i)^2 \leq (\sum\limits_{i=1}^{n} x_{i}^{2})\times(\sum\limits_{i=1}^{n} y_{i}^{2})
$$

**Answer[b]**

Use [Cauchy-Schwarz inequality](https://en.wikipedia.org/wiki/Cauchy%E2%80%93Schwarz_inequality), then

$$
\begin{aligned}
\sum\limits_{i=1}^{n}(x_i+y_i)^2 &= \sum\limits_{i=1}^{n} x_i^2 + \sum\limits_{i=1}^{n} y_i^2 + 2\sum\limits_{i=1}^{n} x_iy_i\\
&\leq \sum\limits_{i=1}^{n} x_i^2 + \sum\limits_{i=1}^{n} y_i^2 + 2\sqrt{(\sum\limits_{i=1}^{n} x_i^2)\times(\sum\limits_{i=1}^{n} y_i^2)}\\
&=\Bigg(\sqrt{\sum\limits_{i=1}^{n} x_{i}^{2}}+\sqrt{\sum\limits_{i=1}^{n} y_{i}^{2}}\;\Bigg)^2
\end{aligned}
$$